Save point of DTree. The only admitted lemma is to show that reachablity analysis is sound.
git-svn-id: https://webdav.seas.upenn.edu/svn/sol/vol@3401 eef5ea85-cc2e-0410-bd84-0fae1f012da8

src/Transforms/dtree.v
@@ -155,52 +155,622 @@ match dt with
 end.
 
 (* l1 >> l2, l1 strict dominates l2 *)
-Definition gt_sdom (res: AMap.t (set l)) (l1 l2:l) : bool :=
+Definition gt_sdom bd (res: AMap.t (Dominators.t bd)) (l1 l2:l) : bool :=
 match AMap.get l2 res with
-| dts2 => in_dec l_dec l1 dts2
+| Dominators.mkBoundedSet dts2 _ => in_dec l_dec l1 dts2
 end.
 
-Fixpoint find_min (res: AMap.t (set l)) (acc:l) (dts: set l): l :=
+Fixpoint find_min bd (res: AMap.t (Dominators.t bd)) (acc:l) (dts: set l): l :=
 match dts with
 | nil => acc
 | l0::dts' =>
-    if (gt_sdom res acc l0) then
-      find_min res l0 dts' 
+    if (gt_sdom bd res acc l0) then
+      find_min bd res l0 dts' 
     else
-      find_min res acc dts' 
+      find_min bd res acc dts' 
 end.
 
-Fixpoint insert_sdom_iter (res: AMap.t (set l)) (l0:l) (prefix suffix:list l) 
-  : list l :=
+Fixpoint insert_sort_sdom_iter bd (res: AMap.t (Dominators.t bd)) (l0:l) 
+  (prefix suffix:list l) : list l :=
 match suffix with
 | nil => List.rev (l0 :: prefix)
 | l1::suffix' => 
-    if gt_sdom res l0 l1 then (List.rev (l0 :: prefix)) ++ suffix
-    else insert_sdom_iter res l0 (l1::prefix) suffix'
+    if gt_sdom bd res l0 l1 then (List.rev (l0 :: prefix)) ++ suffix
+    else insert_sort_sdom_iter bd res l0 (l1::prefix) suffix'
 end.
 
-Fixpoint insert_sort_sdom (res: AMap.t (set l)) (data:list l) (acc:list l) 
-  : list l :=
+Fixpoint insert_sort_sdom bd (res: AMap.t (Dominators.t bd)) (data:list l) 
+  (acc:list l) : list l :=
 match data with
 | nil => acc 
-| l1 :: data' => insert_sort_sdom res data' (insert_sdom_iter res l1 nil acc)
+| l1 :: data' => 
+    insert_sort_sdom bd res data' (insert_sort_sdom_iter bd res l1 nil acc)
 end.
 
-Definition sort_sdom (res: AMap.t (set l)) (data:list l) : list l :=
-insert_sort_sdom res data nil.
+Definition sort_sdom bd (res: AMap.t (Dominators.t bd)) (data:list l): list l :=
+insert_sort_sdom bd res data nil.
 
 Require Import Sorted.
 
-Definition gt_sdom_prop (res: AMap.t (set l)) (l1 l2:l) : Prop :=
-gt_sdom res l1 l2 = true.
+Definition gt_dom_prop bd (res: AMap.t (Dominators.t bd)) (l1 l2:l) : Prop :=
+gt_sdom bd res l1 l2 = true \/ l1 = l2.
 
-Lemma insert_sdom_iter_sorted: forall res input,
-  Sorted (gt_sdom_prop res) (sort_sdom res input).
+Lemma sorted_append: forall A (R:A -> A -> Prop) a (l1:list A),
+  (forall a1 l1', 
+    l1 = l1'++a1::nil -> R a1 a) ->
+  Sorted R l1 -> Sorted R (l1 ++ a :: nil).
+Proof.
+  induction l1; intros; simpl; auto.
+    inv H0.
+    constructor; auto.
+      apply IHl1; auto.
+        intros. subst. 
+        apply H with (l1'0:=a0 :: l1'); auto.
+      inv H4; simpl; auto.
+      constructor.
+        apply H with (l1':=nil); auto.
+Qed.
+
+Lemma HdRel_insert: forall A (R:A -> A -> Prop) a a0 l2 l1
+  (H : forall (a1 : A) (l1' : list A), a :: l1 = l1' ++ a1 :: nil -> R a1 a0)
+  (H5 : HdRel R a (l1 ++ l2)),
+  HdRel R a (l1 ++ a0 :: l2).
+Proof.
+  induction l1; simpl; intros.
+    constructor.
+      apply H with (l1':=nil); auto.
+    inv H5. constructor; auto.
+Qed.  
+
+Lemma sorted_insert: forall A (R:A -> A -> Prop) (l2 l1:list A) a,
+  (forall a1 l1', l1 = l1'++a1::nil -> R a1 a) ->
+  (forall a2 l2', l2 = a2::l2' -> R a a2) ->
+  Sorted R (l1 ++ l2) -> Sorted R (l1 ++ a :: l2).
+Proof.
+  induction l1; simpl; intros.
+    constructor; auto.
+      destruct l2; constructor.
+        eapply H0; eauto.
+
+    inv H1.
+    constructor.
+      apply IHl1; auto.
+        intros. subst.
+        apply H with (l1'0:=a::l1'); eauto.
+        apply HdRel_insert; auto.
+Qed.
+
+Lemma In_bound_fdef__blockInFdefB: forall f l3,
+  In l3 (bound_fdef f) -> 
+  exists ps, exists cs, exists tmn, 
+    blockInFdefB (block_intro l3 ps cs tmn) f = true.
 Admitted.
 
-Lemma insert_sdom_iter_safe: forall res input l0,
-  In l0 input <-> In l0 (sort_sdom res input).
-Admitted.
+Lemma gt_dom_prop_trans : forall ifs S M f l1 l2 l3
+  (HwfF: wf_fdef ifs S M f) (Huniq: uniqFdef f)
+  (HBinF1: In l1 (bound_fdef f))
+  (HBinF2: In l2 (bound_fdef f))
+  (HBinF3: In l3 (bound_fdef f))
+  (H1 : gt_dom_prop (bound_fdef f) (dom_analyze f) l1 l2)
+  (H2 : gt_dom_prop (bound_fdef f) (dom_analyze f)  l2 l3),
+  gt_dom_prop (bound_fdef f) (dom_analyze f) l1 l3.
+Proof.
+  unfold gt_dom_prop, gt_sdom.
+  intros.
+  remember (Maps.AMap.get l2 (dom_analyze f)) as R2.
+  remember (Maps.AMap.get l3 (dom_analyze f)) as R3.
+  destruct R2. destruct R3.
+  apply In_bound_fdef__blockInFdefB in HBinF1. 
+  apply In_bound_fdef__blockInFdefB in HBinF2. 
+  apply In_bound_fdef__blockInFdefB in HBinF3. 
+  destruct HBinF1 as [ps1 [cs1 [tmn1 HBinF1]]].
+  destruct HBinF2 as [ps2 [cs2 [tmn2 HBinF2]]].
+  destruct HBinF3 as [ps3 [cs3 [tmn3 HBinF3]]].
+  destruct (l_dec l1 l3); auto.
+  destruct H2 as [H2 | H2]; subst; auto.
+  Case "l2 in sdom(l3)".
+    destruct (in_dec l_dec l2 bs_contents0); inv H2.
+    left.
+    assert (domination f l2 l3) as Hdom23.
+      eapply dom_is_sound; eauto.
+        rewrite <- HeqR3. simpl. auto.
+    destruct H1 as [H1 | H1]; subst.
+    SCase "l1 in sdom(l2)".
+      destruct (in_dec l_dec l1 bs_contents); inv H1.
+      assert (domination f l1 l2) as Hdom12.
+        eapply dom_is_sound; eauto.
+          rewrite <- HeqR2. simpl. auto.
+      assert (strict_domination f l1 l3) as Hsdom13.
+        split; auto.
+          eapply dom_tran; eauto.
+      eapply sdom_is_complete in Hsdom13; eauto.
+        rewrite <- HeqR3 in Hsdom13. simpl in *. 
+        destruct (in_dec l_dec l1 bs_contents0); auto.
+
+        rewrite <- HeqR3. simpl. 
+        destruct bs_contents0; auto.
+          intro J. inv J.
+
+    SCase "l1=l2".
+      assert (strict_domination f l2 l3) as Hsdom23.
+        split; auto.
+      eapply sdom_is_complete in Hsdom23; eauto.
+        destruct (in_dec l_dec l2 bs_contents0); auto.
+
+        rewrite <- HeqR3. simpl. 
+        destruct bs_contents0; auto.
+          intro J. inv J.
+
+  Case "l2=l3".
+    rewrite <- HeqR3 in HeqR2. inv HeqR2; auto.
+Qed.
+
+Lemma gt_sdom_prop_trans : forall ifs S M f l1 l2 l3
+  (HwfF: wf_fdef ifs S M f) (Huniq: uniqFdef f)
+  (HBinF1: In l1 (bound_fdef f))
+  (HBinF2: In l2 (bound_fdef f))
+  (HBinF3: In l3 (bound_fdef f))
+  (H1 : gt_sdom (bound_fdef f) (dom_analyze f) l1 l2 = true)
+  (H2 : gt_sdom (bound_fdef f) (dom_analyze f)  l2 l3 = true),
+  gt_sdom (bound_fdef f) (dom_analyze f)  l1 l3 = true.
+Proof.
+  unfold gt_sdom.
+  intros. 
+  remember (Maps.AMap.get l2 (dom_analyze f)) as R1.
+  remember (Maps.AMap.get l3 (dom_analyze f)) as R2.
+  destruct R1. destruct R2.
+  destruct (in_dec l_dec l2 bs_contents0); inv H2.
+  destruct (in_dec l_dec l1 bs_contents); inv H1.
+  apply In_bound_fdef__blockInFdefB in HBinF1. 
+  apply In_bound_fdef__blockInFdefB in HBinF2. 
+  apply In_bound_fdef__blockInFdefB in HBinF3. 
+  destruct HBinF1 as [ps1 [cs1 [tmn1 HBinF1]]].
+  destruct HBinF2 as [ps2 [cs2 [tmn2 HBinF2]]].
+  destruct HBinF3 as [ps3 [cs3 [tmn3 HBinF3]]].
+  destruct (reachable_dec f l3).
+    assert (strict_domination f l2 l3) as Hsdom23.
+      eapply sdom_is_sound; eauto.
+        rewrite <- HeqR2. simpl. auto.
+    assert (reachable f l2) as Hreach2.
+      apply sdom_reachable in Hsdom23; auto.
+    assert (strict_domination f l1 l2) as Hsdom12.
+      eapply sdom_is_sound; eauto.
+        rewrite <- HeqR1. simpl. auto.
+    assert (strict_domination f l1 l3) as Hsdom13.
+      eapply sdom_tran with (l2:=l2); eauto.
+    eapply sdom_is_complete in Hsdom13; eauto.
+      rewrite <- HeqR2 in Hsdom13. simpl in *. 
+      destruct (in_dec l_dec l1 bs_contents0); auto.
+
+      rewrite <- HeqR2. simpl. 
+      destruct bs_contents0; auto.
+        intro J. inv J.
+    
+    eapply dom_unreachable in H; eauto. 
+      rewrite <- HeqR2 in H. simpl in H.
+      destruct H. 
+      apply blockInFdefB_in_vertexes in HBinF1.
+      unfold vertexes_fdef in HBinF1. 
+      apply H0 in HBinF1.
+      destruct (in_dec l_dec l1 bs_contents0); auto.
+
+      rewrite <- HeqR2. simpl. intro J. subst. inv i0.
+Qed.
+
+(*
+Lemma sdom_ordered : forall f l1 l2 l3
+  (Hneq: l1 <> l2) (Hreach: reachable f l3)
+  (Hsdom: strict_domination f l1 l3)
+  (Hsdom': strict_domination f l2 l3),
+  strict_domination f l1 l2 \/ strict_domination f l2 l1.
+
+Lemma sdom_is_sound : forall
+  ifs S M (f : fdef) (l3 : l) (l' : l) ps cs tmn
+  (HwfF : wf_fdef ifs S M f) (HuniqF : uniqFdef f) (Hreach : reachable f l3)
+  (HBinF : blockInFdefB (block_intro l3 ps cs tmn) f = true)
+  (Hin : 
+    In l' (DomDS.L.bs_contents _ ((dom_analyze f) !! l3))),
+  strict_domination f l' l3.
+Proof. 
+Lemma sdom_is_complete: forall
+  ifs S M (f : fdef) (l3 : l) (l' : l) ps cs tmn ps' cs' tmn'
+  (HwfF : wf_fdef ifs S M f) (HuniqF : uniqFdef f)
+  (HBinF' : blockInFdefB (block_intro l' ps' cs' tmn') f = true)
+  (HBinF : blockInFdefB (block_intro l3 ps cs tmn) f = true)
+  (Hsdom: strict_domination f l' l3)
+  (Hnempty: DomDS.L.bs_contents _ ((dom_analyze f) !! l3) <> nil),
+  In l' (DomDS.L.bs_contents _ ((dom_analyze f) !! l3)).
+Proof.
+
+*)
+
+Definition getEntryLabel (f:fdef) : option l :=
+match f with
+| fdef_intro _ ((block_intro l0 _ _ _)::_) => Some l0
+| _ => None
+end.
+
+Lemma dom_analysis__entry_doms_others1: forall ifs S M f 
+  (HwfF: wf_fdef ifs S M f) entry
+  (H: getEntryLabel f = Some entry)
+  (Hex: exists b,  match (AMap.get b (dom_analyze f)) with
+                   | Dominators.mkBoundedSet dts _ => dts <> nil
+                   end),
+  (forall b, b <> entry /\ reachable f b ->
+     match (AMap.get b (dom_analyze f)) with
+     | Dominators.mkBoundedSet dts _ => In entry dts
+     end).
+Proof.
+  intros.
+  destruct H0 as [J1 J2].
+  case_eq ((dom_analyze f) !! b).
+  intros bs_contents bs_bound H1.
+  unfold dom_analyze in H1, Hex.
+  destruct f.
+  remember (entry_dom b0) as R.
+  destruct R. 
+  destruct x as [[]|]; subst.
+    destruct b0; inv H.
+    destruct b1; tinv y.
+    destruct bs_contents0; tinv y.
+    destruct b0. inv HeqR.
+    inv H2. 
+    remember (
+      DomDS.fixpoint (bound_blocks (block_intro entry p c t :: b2))
+           (successors_blocks (block_intro entry p c t :: b2))
+           (transfer (bound_blocks (block_intro entry p c t :: b2)))
+           ((entry,
+            {| DomDS.L.bs_contents := nil; DomDS.L.bs_bound := bs_bound0 |})
+            :: nil)) as R.
+    destruct R.
+      symmetry in HeqR.
+      eapply EntryDomsOthers.dom_entry_doms_others with (entry:=entry) in HeqR; 
+        eauto.
+        unfold EntryDomsOthers.entry_doms_others in HeqR.
+        apply HeqR in J1.
+        unfold Dominators.member in J1.
+        unfold EntryDomsOthers.dt, EntryDomsOthers.bound, DomDS.dt, DomDS.L.t 
+          in J1. 
+        unfold Dominators.t in H1. simpl in J1, H1.
+        rewrite H1 in J1; auto.
+
+        split. 
+           remember (Kildall.successors_list
+             (EntryDomsOthers.predecessors (block_intro entry p c t :: b2)) 
+               entry) as R.
+           destruct R; auto.
+           assert (
+             In a 
+               (Kildall.successors_list
+                 (EntryDomsOthers.predecessors (block_intro entry p c t :: b2)) 
+               entry)) as Hin. rewrite <- HeqR0. simpl; auto.
+           apply Kildall.make_predecessors_correct' in Hin.
+           change (successors_blocks (block_intro entry p c t :: b2)) with
+             (successors (fdef_intro f (block_intro entry p c t :: b2))) in Hin.
+           apply successors__blockInFdefB in Hin.
+           destruct Hin as [ps0 [cs0 [tmn0 [G1 G2]]]].
+           eapply getEntryBlock_inv with (l3:=a)(a:=entry) in G2; simpl; eauto.
+           congruence.
+
+        split; auto.
+          exists{| DomDS.L.bs_contents := nil; DomDS.L.bs_bound := bs_bound0 |}.
+          simpl.
+          split; auto.
+            split; intros x Hin; auto.
+
+      rewrite AMap.gso in H1; auto.
+      rewrite AMap.gi in H1. inv H1.
+      destruct Hex as [b0 Hex]. 
+      destruct (l_dec entry b0); subst.
+        rewrite AMap.gss in Hex; auto. congruence.
+
+        rewrite AMap.gso in Hex; auto. rewrite AMap.gi in Hex. simpl in Hex.
+        contradict Hex; auto.
+
+    inv H.
+Qed.
+
+Lemma gt_dom_dec_aux: forall ifs S M f (HwfF: wf_fdef ifs S M f) 
+  (Huniq: uniqFdef f) l1 l2 l3
+  (Hreach: reachable f l3)
+  (HBinF1: In l1 (bound_fdef f))
+  (HBinF2: In l2 (bound_fdef f))
+  (HBinF3: In l3 (bound_fdef f)),
+  gt_sdom (bound_fdef f) (dom_analyze f) l1 l3 ->
+  gt_sdom (bound_fdef f) (dom_analyze f) l2 l3 ->
+  gt_dom_prop (bound_fdef f) (dom_analyze f) l1 l2 \/ 
+  gt_dom_prop (bound_fdef f) (dom_analyze f) l2 l1.
+Proof.
+  unfold gt_dom_prop, gt_sdom. intros.
+  destruct (l_dec l1 l2); auto.
+  remember ((dom_analyze f) !! l3 ) as R3.
+  remember ((dom_analyze f) !! l2 ) as R2.
+  remember ((dom_analyze f) !! l1 ) as R1.
+  destruct R1, R2, R3.
+  destruct (in_dec l_dec l1 bs_contents1); inv H.
+  destruct (in_dec l_dec l2 bs_contents1); inv H0.
+  apply In_bound_fdef__blockInFdefB in HBinF1. 
+  apply In_bound_fdef__blockInFdefB in HBinF2. 
+  apply In_bound_fdef__blockInFdefB in HBinF3. 
+  destruct HBinF1 as [ps1 [cs1 [tmn1 HBinF1]]].
+  destruct HBinF2 as [ps2 [cs2 [tmn2 HBinF2]]].
+  destruct HBinF3 as [ps3 [cs3 [tmn3 HBinF3]]].
+  assert (strict_domination f l1 l3) as Hsdom13.
+    eapply sdom_is_sound; eauto.
+      rewrite <- HeqR3. simpl. auto.
+  assert (strict_domination f l2 l3) as Hsdom23.
+    eapply sdom_is_sound; eauto.
+      rewrite <- HeqR3. simpl. auto.
+  assert (exists entry, getEntryLabel f = Some entry) as Hentry.
+    inv HwfF. clear - H4. simpl in *.
+    destruct blocks5; inv H4. destruct block5. eauto.
+  destruct Hentry as [entry Hentry].
+  assert (exists b : atom,
+     match (dom_analyze f) !! b with
+     | {| DomDS.L.bs_contents := dts |} => dts <> nil
+     end) as Hex.
+    exists l3. rewrite <- HeqR3. intro J. subst. inv i1.
+  assert (reachable f l2) as Hreach2.
+    apply sdom_reachable in Hsdom23; auto.
+  assert (reachable f l1) as Hreach1.
+    apply sdom_reachable in Hsdom13; auto.
+  destruct (l_dec l1 entry); subst.
+    left. left.
+    assert (    
+      match (AMap.get l2 (dom_analyze f)) with
+      | Dominators.mkBoundedSet dts _ => In entry dts
+      end) as G.
+      eapply dom_analysis__entry_doms_others1; eauto.
+        rewrite <- HeqR2 in G. 
+        destruct (in_dec l_dec entry bs_contents0); auto.
+  destruct (l_dec l2 entry); subst.
+    right. left.
+    assert (    
+      match (AMap.get l1 (dom_analyze f)) with
+      | Dominators.mkBoundedSet dts _ => In entry dts
+      end) as G.
+      eapply dom_analysis__entry_doms_others1; eauto.
+        rewrite <- HeqR1 in G. 
+        destruct (in_dec l_dec entry bs_contents); auto.
+  eapply sdom_ordered with (l1:=l2) in Hsdom13; eauto.
+  destruct Hsdom13 as [Hsdom21 | Hsdom12].
+    right.
+    eapply sdom_is_complete in Hsdom21; eauto.
+      rewrite <- HeqR1 in Hsdom21. simpl in Hsdom21.
+      destruct (in_dec l_dec l2 bs_contents); simpl; auto.
+
+      rewrite <- HeqR1. simpl. 
+      assert (    
+        match (AMap.get l1 (dom_analyze f)) with
+        | Dominators.mkBoundedSet dts _ => In entry dts
+        end) as G.
+        eapply dom_analysis__entry_doms_others1; eauto.
+          rewrite <- HeqR1 in G. intro J. subst. inv G.
+
+    left.
+    eapply sdom_is_complete in Hsdom12; eauto.
+      rewrite <- HeqR2 in Hsdom12. simpl in Hsdom12.
+      destruct (in_dec l_dec l1 bs_contents0); simpl; auto.
+
+      rewrite <- HeqR2. simpl.
+      assert (    
+        match (AMap.get l2 (dom_analyze f)) with
+        | Dominators.mkBoundedSet dts _ => In entry dts
+        end) as G.
+        eapply dom_analysis__entry_doms_others1; eauto.
+          rewrite <- HeqR2 in G. intro J. subst. inv G.
+Qed.
+
+Lemma gt_dom_dec: forall ifs S M f (HwfF: wf_fdef ifs S M f) 
+  (Huniq: uniqFdef f) l1 l2 l3
+  (Hreach: reachable f l3)
+  (HBinF1: In l1 (bound_fdef f))
+  (HBinF2: In l2 (bound_fdef f))
+  (HBinF3: In l3 (bound_fdef f)),
+  gt_dom_prop (bound_fdef f) (dom_analyze f) l1 l3 ->
+  gt_dom_prop (bound_fdef f) (dom_analyze f) l2 l3 ->
+  gt_dom_prop (bound_fdef f) (dom_analyze f) l1 l2 \/ 
+  gt_dom_prop (bound_fdef f) (dom_analyze f) l2 l1.
+Proof.
+  intros.
+  destruct H as [H | H]; subst; auto.
+  destruct H0 as [H0 | H0]; subst.
+    eapply gt_dom_dec_aux; eauto.
+    left. left. auto.
+Qed.
+
+Lemma gt_sdom_dec: forall ifs S M f (HwfF: wf_fdef ifs S M f) 
+  (Huniq: uniqFdef f) l1 l2 l3
+  (Hneq: l1 <> l2)
+  (Hreach: reachable f l3)
+  (HBinF1: In l1 (bound_fdef f))
+  (HBinF2: In l2 (bound_fdef f))
+  (HBinF3: In l3 (bound_fdef f)),
+  gt_sdom (bound_fdef f) (dom_analyze f) l1 l3 ->
+  gt_sdom (bound_fdef f) (dom_analyze f) l2 l3 ->
+  gt_sdom (bound_fdef f) (dom_analyze f) l1 l2 \/ 
+  gt_sdom (bound_fdef f) (dom_analyze f) l2 l1.
+Proof.
+  intros.
+  apply gt_dom_dec with (l1:=l1) (l2:=l2) (l3:=l3) in HwfF; auto.
+    destruct HwfF as [[J | J] | [J | J]]; subst; auto; try congruence.
+    left. auto.
+    left. auto.
+Qed.
+
+Lemma insert_sort_sdom_iter_safe: forall bd res l0 suffix l1 prefix,
+  (In l0 (prefix ++ suffix) \/ l0 = l1) <->
+  In l0 (insert_sort_sdom_iter bd res l1 prefix suffix).
+Proof.
+  induction suffix; simpl; intros.
+    split; intro J.
+      apply in_or_app.
+      destruct J as [J | J]; subst.
+        left. simpl_env in J. apply in_rev in J; auto.
+        right. simpl. auto.
+
+      apply in_app_or in J. simpl in J. simpl_env.
+      destruct J as [J | [J | J]]; subst; auto.
+        left. apply in_rev in J; auto.
+        tauto.
+
+    simpl_env. simpl.
+    split; intro J.
+      destruct (gt_sdom bd res l1 a).
+        destruct J as [J | J]; subst.
+          apply in_app_or in J. simpl in J.
+          apply in_or_app. simpl.
+          destruct J as [J | [J | J]]; subst; auto.
+            apply in_rev in J; auto.
+
+          apply in_or_app. simpl. auto.
+        apply IHsuffix.
+          destruct J as [J | J]; auto.
+          left. simpl.         
+          apply in_app_or in J. simpl in J.
+          destruct J as [J | [J | J]]; subst; auto.
+            right. apply in_or_app; auto.
+            right. apply in_or_app; auto.
+
+      destruct (gt_sdom bd res l1 a).
+        apply in_app_or in J. simpl in J.
+        destruct J as [J | [J | [J | J]]]; subst; auto.
+          left. apply in_or_app. simpl.
+          apply in_rev in J; auto.
+
+          left. apply in_or_app. simpl. auto.
+          left. apply in_or_app. simpl. auto.
+        apply IHsuffix in J.
+          destruct J as [J | J]; auto.
+          left. apply in_or_app. simpl.
+          apply in_app_or in J. simpl in J.
+          destruct J as [[J | J] | J]; subst; auto.
+Qed.
+
+Lemma insert_sort_sdom_safe: forall bd res data acc l0,
+  (In l0 acc \/ In l0 data) <-> In l0 (insert_sort_sdom bd res data acc).
+Proof.
+  induction data; simpl; intros; auto.
+    split; tauto.
+
+    split; intro.
+      apply IHdata.
+      destruct H as [H | [H | H]]; subst; auto.
+        left.
+        apply insert_sort_sdom_iter_safe; auto.
+
+        left.
+        apply insert_sort_sdom_iter_safe; auto.
+
+      apply IHdata in H.
+      destruct H as [H | H]; auto.
+      apply insert_sort_sdom_iter_safe in H.
+      destruct H; auto.
+Qed.
+
+Lemma sort_sdom_safe: forall bd res input l0,
+  In l0 (sort_sdom bd res input) <-> In l0 input.
+Proof.
+  intros.
+  unfold sort_sdom.
+  destruct (@insert_sort_sdom_safe bd res input nil l0) as [J1 J2].
+  split; intro; auto.
+    apply J2 in H. destruct H as [H | H]; auto. inv H.
+Qed.
+
+Lemma insert_sort_sdom_iter_sorted: forall ifs S M f (HwfF: wf_fdef ifs S M f) 
+  (Huniq: uniqFdef f) l3 (Hin3: In l3 (bound_fdef f)) (Hreach: reachable f l3)
+  l0 (Hin0: In l0 (bound_fdef f)) 
+  (Hsd03: gt_dom_prop (bound_fdef f) (dom_analyze f) l0 l3) suffix prefix
+  (G: forall l', In l' (prefix ++ suffix) -> 
+      gt_dom_prop (bound_fdef f) (dom_analyze f) l' l3 /\ In l' (bound_fdef f)),
+  Sorted (gt_dom_prop (bound_fdef f) (dom_analyze f)) 
+    (List.rev prefix ++ suffix) ->
+  (forall l1 prefix', prefix = l1 :: prefix' -> 
+      gt_dom_prop (bound_fdef f) (dom_analyze f) l1 l0) ->
+  Sorted (gt_dom_prop (bound_fdef f) (dom_analyze f)) 
+    (insert_sort_sdom_iter (bound_fdef f) (dom_analyze f) l0 prefix suffix).
+Proof.
+  induction suffix; simpl; intros.
+    simpl_env in *.
+    apply sorted_append; auto.
+      intros.
+      apply H0 with (prefix':=rev l1'); auto.
+        rewrite <- rev_involutive at 1.
+        rewrite H1. rewrite rev_unit. auto.
+
+    remember (gt_sdom (bound_fdef f) (dom_analyze f) l0 a) as R.
+    destruct R.
+      simpl_env. simpl.
+      apply sorted_insert; auto.   
+        intros.
+        apply H0 with (prefix':=rev l1'); auto.
+          rewrite <- rev_involutive at 1.
+          rewrite H1. rewrite rev_unit. auto.
+ 
+        intros.
+        inv H1.
+        unfold gt_dom_prop. auto.
+
+      apply IHsuffix.
+        intros. apply G.
+        apply in_or_app. simpl.
+        apply in_app_or in H1. simpl in H1.
+        destruct H1 as [[H1 | H1] | H1]; auto.
+
+        simpl. simpl_env. simpl. auto.
+
+        intros. inv H1.
+        assert (gt_dom_prop (bound_fdef f) (dom_analyze f) l1 l0 \/ 
+                gt_dom_prop (bound_fdef f) (dom_analyze f) l0 l1) as J.
+          assert (In l1 (prefix'++l1::suffix)) as Hin1. apply in_middle.
+          apply G in Hin1. destruct Hin1 as [J1 J2].
+          eapply gt_dom_dec; eauto.
+        destruct J; auto.
+        unfold gt_dom_prop in H1. unfold gt_dom_prop.
+        destruct (l_dec l0 l1); auto.
+        destruct H1 as [H1 | H1]; auto.
+        rewrite <- HeqR in H1. congruence.
+Qed.
+
+Lemma insert_sort_sdom_sorted: forall ifs S M f (HwfF: wf_fdef ifs S M f) 
+  (Huniq: uniqFdef f) l3 (Hin3: In l3 (bound_fdef f)) (Hreach: reachable f l3)
+  data acc
+  (G: forall l', In l' (data++acc) -> 
+      gt_dom_prop (bound_fdef f) (dom_analyze f) l' l3 /\ In l' (bound_fdef f)),
+  Sorted (gt_dom_prop (bound_fdef f) (dom_analyze f)) acc ->
+  Sorted (gt_dom_prop (bound_fdef f) (dom_analyze f)) 
+         (insert_sort_sdom (bound_fdef f) (dom_analyze f) data acc).
+Proof.
+  induction data; simpl; intros; auto.
+    apply IHdata.
+      intros. apply G.
+      apply in_app_or in H0.
+      destruct H0 as [H0 | H0].
+        right. apply in_or_app; auto.
+        apply insert_sort_sdom_iter_safe in H0.
+        destruct H0 as [H0 | H0]; auto.
+          right. apply in_or_app. simpl_env in H0. auto.
+
+      assert (a = a \/ In a (data++acc)) as Hin. auto.
+      apply G in Hin. destruct Hin as [J1 J2].
+      eapply insert_sort_sdom_iter_sorted with (l3:=l3); eauto.
+        intros. apply G. right. apply in_or_app. simpl_env in H0. auto.
+
+        intros. inv H0.
+Qed.
+
+Lemma sort_sdom_sorted: forall ifs S M f (HwfF: wf_fdef ifs S M f) 
+  (Huniq: uniqFdef f) l3 (Hin3: In l3 (bound_fdef f)) (Hreach: reachable f l3)
+  input
+  (G: forall l', In l' input -> 
+      gt_dom_prop (bound_fdef f) (dom_analyze f) l' l3 /\ In l' (bound_fdef f)),
+  Sorted (gt_dom_prop (bound_fdef f) (dom_analyze f)) 
+         (sort_sdom (bound_fdef f) (dom_analyze f) input).
+Proof.
+  intros. unfold sort_sdom.
+  eapply insert_sort_sdom_sorted; simpl_env; eauto.
+Qed.
 
 Fixpoint remove_redundant (input: list l) : list l :=
 match input with
@@ -210,92 +780,663 @@ match input with
 | _ => input
 end.
 
-Lemma remove_redundant_safe: forall input l0,
-  In l0 input <-> In l0 (remove_redundant input).
-Admitted.
+Lemma remove_redundant_safe: forall l0 input,
+  In l0 (remove_redundant input) <-> In l0 input.
+Proof.
+  induction input; simpl.
+    split; auto.
+
+    destruct input.
+      simpl. split; auto.  
+
+      destruct IHinput as [J1 J2].
+      destruct (l_dec a l1); subst.
+        split; intros.
+          apply J1 in H.
+            simpl in H. simpl.
+            destruct H; auto.           
+
+          apply J2.
+            simpl in H. simpl.
+            destruct H as [H | [H | H]]; auto.
+
+        split; intros.
+          Local Opaque remove_redundant. 
+          simpl in H.
+          destruct H as [H | H]; auto.
+
+          simpl.
+          destruct H as [H | H]; auto.
+          Transparent remove_redundant.
+Qed.
+
+Lemma remove_redundant_HdRel: forall R a input,
+  HdRel R a input ->
+  HdRel R a (remove_redundant input).
+Proof.
+  induction input; simpl; intros; auto.
+    destruct input; auto.
+      inv H.
+      destruct (l_dec a0 l0); subst.
+        apply IHinput. apply HdRel_cons; auto. 
+        apply HdRel_cons; auto.
+Qed.
+
+Lemma remove_redundant_In: forall a input,
+  In a (remove_redundant input) -> In a input.
+Proof.
+  induction input; simpl; intros; auto.
+    destruct input; auto.
+      destruct (l_dec a0 l0); subst.
+        apply IHinput in H; auto. 
+
+        Local Opaque remove_redundant. 
+        simpl in H.
+        destruct H as [H | H]; auto.
+        Transparent remove_redundant.
+Qed.
 
 Lemma remove_redundant_sorted: forall R input,
-  Sorted R input ->
-  Sorted R (remove_redundant input) /\ NoDup (remove_redundant input).
-Admitted.
+  Sorted R input -> Sorted R (remove_redundant input).
+Proof.
+  induction input; intros; simpl; auto.
+    destruct input; auto.
+      inv H. 
+      apply IHinput in H2.
+      destruct (l_dec a l0); subst; auto.
+        apply Sorted_cons; auto.
+          apply remove_redundant_HdRel; auto. 
+Qed.
 
-Fixpoint compute_sdom_chains_aux (res: AMap.t (set l)) (bd: list l) 
-  (acc: list (l * list l)) : list (l * list l) :=
+Lemma remove_redundant_NoDup: forall (R:l -> l -> Prop) input
+  (P0:forall a b c, 
+        In a input -> 
+        In b input -> 
+        In c input -> a <> b -> R a b -> R b c -> a <> c),
+  StronglySorted R input ->
+  NoDup (remove_redundant input).
+Proof.
+  induction input; intros; simpl; auto.
+    destruct input; auto.  
+      inv H. 
+      assert (H2':=H2).
+      apply IHinput in H2.
+        destruct (l_dec a l0); subst; auto.
+          apply NoDup_cons; auto.
+          intro J.
+          apply remove_redundant_In in J.
+          simpl in J. 
+          destruct J as [J | J]; subst.
+            congruence.
+
+            eapply Forall_forall with (x:=l0) in H3; simpl; eauto.
+            inv H2'.
+            eapply Forall_forall with (x:=a) in H4; eauto.
+            apply P0 with (c:=a) in H3; simpl; auto.
+
+        intros. apply P0 with (b:=b); simpl; auto.
+Qed.
+
+Lemma remove_redundant_NoDup': forall R input
+  (P0:forall a, In a input -> ~ R a a),
+  StronglySorted R input ->
+  NoDup (remove_redundant input).
+Proof.
+  induction input; intros; simpl; auto.
+    destruct input; auto.  
+      inv H. 
+      apply IHinput in H2.
+        destruct (l_dec a l0); subst; auto.
+          apply NoDup_cons; auto.
+          intro J.
+          apply remove_redundant_In in J.
+          eapply Forall_forall in H3; eauto.
+          revert H3. apply P0. simpl. auto.
+        intros. apply P0. simpl. simpl in H.
+        destruct H; auto.
+Qed.
+
+Fixpoint compute_sdom_chains_aux bd0 (res: AMap.t (Dominators.t bd0))
+  (bd: list l) (acc: list (l * list l)) : list (l * list l) :=
 match bd with
 | nil => acc
 | l0 :: bd' => 
-    compute_sdom_chains_aux res bd' 
-      ((l0, remove_redundant (sort_sdom res (l0 :: AMap.get l0 res)))::acc)
-end.
-
-Definition compute_sdom_chains (res: AMap.t (set l)) (bd: list l) 
-  : list (l * list l) :=
-compute_sdom_chains_aux res bd nil.
-
-Lemma compute_sdom_chains_sorted: forall res bd l0 chain,
-  In (l0, chain) (compute_sdom_chains res bd) ->
-  Sorted (gt_sdom_prop res) chain /\ NoDup chain.
-Admitted.
-
-Lemma compute_sdom_chains_safe: forall res bd l0 chain l1,
-  In (l0, chain) (compute_sdom_chains res bd) ->
-  (In l1 chain <-> In l1 (l0 :: AMap.get l0 res)).
-Admitted.
-
-Fixpoint dep_doms__nondep_doms_aux bd0 (res: AMap.t (Dominators.t bd0)) 
-  bd (acc: AMap.t (set l)) : AMap.t (set l) :=
-match bd with
-| nil => acc
-| l0::bd' => 
     match AMap.get l0 res with
-    | (Dominators.mkBoundedSet dts0 _) =>
-        AMap.set l0 dts0 (dep_doms__nondep_doms_aux bd0 res bd' acc)
+    | Dominators.mkBoundedSet dts0 _ =>
+        compute_sdom_chains_aux bd0 res bd' 
+          ((l0, remove_redundant (sort_sdom bd0 res (l0 :: dts0)))::acc)
     end
 end.
 
-Definition dep_doms__nondep_doms bd (res: AMap.t (Dominators.t bd)) 
-  : AMap.t (set l) :=
-dep_doms__nondep_doms_aux bd res bd (AMap.init nil).
+Definition compute_sdom_chains bd (res: AMap.t (Dominators.t bd)) rd
+  : list (l * list l) :=
+compute_sdom_chains_aux bd res rd nil.
+
+Lemma reachablity_analysis__reachable: forall f rd a,
+  reachablity_analysis f = Some rd -> In a rd -> reachable f a.
+Admitted.
+
+Lemma reachable__in_bound: forall f a,
+  reachable f a ->
+  In a (bound_fdef f).
+Admitted.
+
+Lemma reachablity_analysis__in_bound: forall f rd,
+  reachablity_analysis f = Some rd ->
+  incl rd (bound_fdef f).
+Proof.
+  intros. intros x Hin.
+  apply reachable__in_bound.
+  eapply reachablity_analysis__reachable; eauto.
+Qed.
+
+Lemma gt_sdom_prop_irrefl: forall ifs S M f (HwfF : wf_fdef ifs S M f) 
+  (HuniqF: uniqFdef f) a (Hreach : reachable f a),
+  gt_sdom (bound_fdef f) (dom_analyze f) a a = false. 
+Proof.
+  unfold gt_sdom.
+  intros.
+  remember ((dom_analyze f) !! a) as R.
+  destruct R.
+  assert (J:=Hreach).
+  apply reachable__in_bound in Hreach.
+  apply In_bound_fdef__blockInFdefB in Hreach.
+  destruct Hreach as [ps [cs [tnn HBinF]]].
+  destruct (in_dec l_dec a bs_contents); simpl; auto.
+  eapply sdom_is_sound with (l':=a) in HBinF; eauto.
+    destruct HBinF. congruence.
+    rewrite <- HeqR. auto.
+Qed.
+
+Lemma Sorted_HdRel__Forall: forall A (R : A -> A -> Prop) l0 (H0 : Sorted R l0),
+  forall a : A,
+  (forall x y z : A,
+   In x (a :: l0) ->
+   In y (a :: l0) -> In z (a :: l0) -> R x y -> R y z -> R x z) ->
+  HdRel R a l0 -> Forall (R a) l0.
+Proof.
+  induction l0; simpl; intros.
+    apply Forall_forall.
+    intros. inv H2.
+
+    apply Forall_forall.
+    intros. 
+    simpl in H2.
+    inv H1.
+    destruct H2 as [H2 | H2]; subst; auto.
+    inv H0.
+    apply IHl0 in H6; auto.
+      eapply Forall_forall in H6; eauto.
+      apply H with (y:=a); auto.
+
+      intros.
+      eapply H with (y:=y); simpl; eauto.
+Qed.
+
+Lemma strict_Sorted_StronglySorted : forall A (R:A -> A -> Prop) data,
+  (forall x y z,
+     In x data -> In y data -> In z data -> 
+     R x y -> R y z -> R x z) ->
+  Sorted R data -> StronglySorted R data.
+Proof.
+  intros.
+  induction H0; constructor.
+    apply IHSorted.
+      intros. eapply H with (y:=y); simpl; eauto.
+      apply Sorted_HdRel__Forall in H; auto.
+Qed.
+
+Lemma compute_sdom_chains_aux__dom : forall bd res l0 chain0 rd acc, 
+  In (l0, chain0) (compute_sdom_chains_aux bd res rd acc) -> 
+  In l0 rd \/ In (l0, chain0) acc.
+Proof.
+  induction rd; simpl; intros; auto.
+    destruct (res !! a).
+    apply IHrd in H.
+    destruct H as [H | H]; auto.
+    simpl in H.
+    destruct H as [H | H]; auto.
+    inv H; auto.
+Qed. 
+
+Lemma compute_sdom_chains__dom : forall bd res rd l0 chain0, 
+  In (l0, chain0) (compute_sdom_chains bd res rd) -> In l0 rd.
+Proof.
+  unfold compute_sdom_chains.
+  intros.
+  apply compute_sdom_chains_aux__dom in H.
+  destruct H as [H | H]; auto.
+  inv H.
+Qed.
+
+Lemma compute_sdom_chains_aux_sorted__helper: forall bd0 bd bs_contents res x
+  (bs_bound : incl bs_contents bd0) (l1 : l) (Hinc : incl (l1 :: bd) bd0)
+  (H1 : In x (sort_sdom bd0 res (l1 :: bs_contents))),
+  In x bd0.
+Proof.  
+  intros.
+  apply sort_sdom_safe in H1. 
+  simpl in H1. 
+  destruct H1 as [H1 | H1]; subst.
+    apply Hinc. simpl; auto.
+    apply bs_bound. auto.
+Qed.
+
+Lemma gt_sdom_prop_trans1 : forall ifs S M f l1 l2 l3
+  (HwfF: wf_fdef ifs S M f) (Huniq: uniqFdef f) (Hreach: reachable f l3)
+  (HBinF1: In l1 (bound_fdef f))
+  (HBinF2: In l2 (bound_fdef f))
+  (HBinF3: In l3 (bound_fdef f))
+  (H1 : gt_sdom (bound_fdef f) (dom_analyze f) l1 l2 = true)
+  (H2 : gt_dom_prop (bound_fdef f) (dom_analyze f) l2 l3),
+  gt_sdom (bound_fdef f) (dom_analyze f) l1 l3 = true.
+Proof.
+  unfold gt_dom_prop, gt_sdom.
+  intros. 
+  remember (Maps.AMap.get l2 (dom_analyze f)) as R2.
+  remember (Maps.AMap.get l3 (dom_analyze f)) as R3.
+  destruct R2. destruct R3.
+  destruct (in_dec l_dec l1 bs_contents); inv H1.
+  apply In_bound_fdef__blockInFdefB in HBinF1. 
+  apply In_bound_fdef__blockInFdefB in HBinF2. 
+  apply In_bound_fdef__blockInFdefB in HBinF3. 
+  destruct HBinF1 as [ps1 [cs1 [tmn1 HBinF1]]].
+  destruct HBinF2 as [ps2 [cs2 [tmn2 HBinF2]]].
+  destruct HBinF3 as [ps3 [cs3 [tmn3 HBinF3]]].
+  assert (domination f l2 l3) as Hdom23.
+    eapply dom_is_sound; eauto.
+      rewrite <- HeqR3. simpl. 
+      destruct H2 as  [H2 | H2]; auto.
+        destruct (in_dec l_dec l2 bs_contents0); inv H2; auto.
+  assert (reachable f l2) as Hreach2.
+     apply dom_reachable in Hdom23; auto.
+  assert (strict_domination f l1 l2) as Hsdom12.
+    eapply sdom_is_sound; eauto.
+      rewrite <- HeqR2. simpl. auto.
+  eapply sdom_tran1 with (l3:=l3) in Hsdom12; eauto.
+  eapply sdom_is_complete in Hsdom12; eauto.
+    rewrite <- HeqR3 in Hsdom12. simpl in Hsdom12.
+    destruct (in_dec l_dec l1 bs_contents0); auto.
+
+    rewrite <- HeqR3. simpl. 
+    destruct H2 as [H2 | H2]; subst.
+      destruct bs_contents0.
+        inv H2.
+        intro J. inv J.
+
+      rewrite <- HeqR3 in HeqR2. inv HeqR2.
+      destruct bs_contents0.
+        inv i0.
+        intro J. inv J.
+Qed.
+
+Lemma compute_sdom_chains_aux_sorted: forall ifs S M f 
+  (HwfF: wf_fdef ifs S M f) (Huniq: uniqFdef f)
+  l0 chain0 bd (Hinc: incl bd (bound_fdef f)) 
+  (Hreach: forall x, In x bd -> reachable f x) acc,
+  (forall l0 chain0, In (l0, chain0) acc ->
+    Sorted (gt_dom_prop (bound_fdef f) (dom_analyze f)) chain0 /\ 
+    NoDup chain0) ->
+  In (l0, chain0) 
+    (compute_sdom_chains_aux (bound_fdef f) (dom_analyze f) bd acc) ->
+  Sorted (gt_dom_prop (bound_fdef f) (dom_analyze f)) chain0 /\ NoDup chain0.
+Proof.
+  induction bd; simpl; intros; eauto.
+    remember ((dom_analyze f) !! a) as R.
+    destruct R.
+    apply IHbd in H0; auto.
+      simpl_env in Hinc.
+      apply AtomSet.incl_app_invr in Hinc; auto.
+
+      intros.
+      destruct H1 as [H1 | H1]; eauto.
+      inv H1. 
+      assert (In l1 (bound_fdef f)) as G1.
+        apply Hinc; simpl; auto.
+      assert (forall l' : l,
+        In l' (l1 :: bs_contents) ->
+        gt_dom_prop (bound_fdef f) (dom_analyze f) l' l1 /\ In l' (bound_fdef f)) 
+        as G2.
+        intros l' Hin.
+        simpl in Hin.
+        destruct Hin as [EQ | Hin]; subst.
+          unfold gt_dom_prop. split; auto.
+         
+          split.
+            unfold gt_dom_prop, gt_sdom.
+            rewrite <- HeqR. 
+            destruct (in_dec l_dec l' bs_contents); simpl; auto.
+        
+            apply bs_bound; auto.
+      split.
+        apply remove_redundant_sorted; auto.
+          eapply sort_sdom_sorted; eauto.
+
+        apply remove_redundant_NoDup with 
+          (R:=gt_dom_prop (bound_fdef f) (dom_analyze f)); auto.
+          intros.
+          destruct H5; subst; try congruence.
+          assert (reachable f c) as Hreachc. 
+            apply sort_sdom_safe in H3.
+              simpl in H3.
+              destruct H3 as [H3 | H3]; subst.
+                apply Hreach; auto.
+           
+                assert (reachable f l1) as Hreach1. apply Hreach; auto.
+                eapply sdom_reachable; eauto.
+                  assert (In l1 (bound_fdef f)) as Hin.
+                    apply Hinc; simpl; auto.
+                  apply In_bound_fdef__blockInFdefB in Hin.
+                  destruct Hin as [ps [cs [tmn HBinF]]].
+                  eapply sdom_is_sound; eauto.
+                    rewrite <- HeqR. auto.
+          eapply gt_sdom_prop_trans1 with (l1:=a) in H6;
+            eauto using compute_sdom_chains_aux_sorted__helper.
+            intro EQ; subst.
+            apply gt_sdom_prop_irrefl with (a:=c) in HwfF; auto.
+            rewrite HwfF in H6. congruence.
+
+          apply strict_Sorted_StronglySorted.
+            intros.
+            eapply gt_dom_prop_trans with (l2:=y); 
+              eauto using compute_sdom_chains_aux_sorted__helper.
+            eapply sort_sdom_sorted; eauto.
+Qed.
+
+Definition gt_sdom_prop bd (res: AMap.t (Dominators.t bd)) (l1 l2:l) : Prop :=
+gt_sdom bd res l1 l2 = true.
+
+Lemma NoDup_gt_dom_prop_sorted__gt_dsom_prop_sorted: forall f chain
+  (Hsorted: Sorted (gt_dom_prop (bound_fdef f) (dom_analyze f)) chain)
+  (Huniq: NoDup chain),
+  Sorted (gt_sdom_prop (bound_fdef f) (dom_analyze f)) chain.
+Proof.
+  intros.
+  induction Hsorted; simpl; intros; auto.
+    inv Huniq.
+    constructor; auto.  
+      inv H; auto.
+      constructor.
+        destruct H0; subst; auto.
+          contradict H2; simpl; auto.
+Qed.
+
+Lemma compute_sdom_chains_sorted: forall ifs S M f 
+  (HwfF: wf_fdef ifs S M f) (Huniq: uniqFdef f)
+  rd (Hinc: incl rd (bound_fdef f)) (Hreach: forall x, In x rd -> reachable f x) 
+  l0 chain,
+  In (l0, chain) (compute_sdom_chains (bound_fdef f) (dom_analyze f) rd) ->
+  Sorted (gt_sdom_prop (bound_fdef f) (dom_analyze f)) chain /\ NoDup chain.
+Proof.
+  intros.
+  unfold compute_sdom_chains in H.
+  eapply compute_sdom_chains_aux_sorted in H; eauto.
+    destruct H as [H1 H2].
+    split; auto.
+      apply NoDup_gt_dom_prop_sorted__gt_dsom_prop_sorted; auto.
+
+    simpl. intros. tauto.
+Qed. 
+
+Lemma compute_sdom_chains_aux_safe: forall bd0 (res:AMap.t (Dominators.t bd0)) 
+  l0 l1 chain0 dts0 P0 bd acc,
+  (forall l0 l1 chain0 dts0 P0,
+    In (l0, chain0) acc ->
+    AMap.get l0 res = Dominators.mkBoundedSet _ dts0 P0 ->
+    (In l1 chain0 <-> In l1 (l0 :: dts0))) ->
+  In (l0, chain0) (compute_sdom_chains_aux bd0 res bd acc) ->
+  AMap.get l0 res = Dominators.mkBoundedSet _ dts0 P0 ->
+  (In l1 chain0 <-> In l1 (l0 :: dts0)).
+Proof.
+  induction bd; intros; eauto.
+    simpl in H0. 
+    remember (@AMap.get (Dominators.t bd0) a res) as R.
+    destruct R.
+    apply IHbd in H0; auto.
+    intros. simpl in H2.
+    destruct H2 as [H2 | H2]; eauto.
+    inv H2. rewrite H3 in HeqR. inv HeqR.
+    destruct (@remove_redundant_safe l3 (sort_sdom bd0 res (l2 :: dts1)))
+      as [J1 J2].
+    destruct (@sort_sdom_safe bd0 res (l2 :: dts1) l3) as [J3 J4].
+    split; eauto.
+Qed.
+
+Lemma compute_sdom_chains_safe: forall bd res rd l0 chain l1 dts0 P0,
+  In (l0, chain) (compute_sdom_chains bd res rd) ->
+  AMap.get l0 res = Dominators.mkBoundedSet _ dts0 P0 ->
+  (In l1 chain <-> In l1 (l0 :: dts0)).
+Proof.
+  intros.
+  unfold compute_sdom_chains in H.
+  eapply compute_sdom_chains_aux_safe in H; eauto.
+  simpl. intros. tauto.
+Qed. 
 
 Definition wf_chain f dt (chain:list l) : Prop :=
 match chain with
-| entry :: _ => 
+| entry :: _ :: _ => 
    let b := bound_fdef f in
-   let res := dep_doms__nondep_doms b (dom_analyze f) in
+   let res := (dom_analyze f) in
    entry `in` dtree_dom dt /\
-   Sorted (gt_sdom_prop res) chain /\ NoDup chain
-| _ => False
+   Sorted (gt_sdom_prop b res) chain /\ NoDup chain
+| _ => True
 end.
 
-Definition getEntryLabel (f:fdef) : option l :=
-match f with
-| fdef_intro _ ((block_intro l0 _ _ _)::_) => Some l0
-| _ => None
-end.
+Lemma compute_sdom_chains__in_bound: forall l0 chain0 bd res rd
+  (Hinc: incl rd bd),
+  In (l0, chain0) (compute_sdom_chains bd res rd) ->
+  incl chain0 bd.
+Proof.
+  intros.
+  remember (AMap.get l0 res) as R. destruct R.
+  intros x Hin.
+  assert (H':=H).
+  eapply compute_sdom_chains_safe in H; eauto.
+  eapply H in Hin.
+  simpl in Hin.
+  destruct Hin as [Hin | Hin]; subst; auto.
+  apply compute_sdom_chains__dom in H'; auto.
+Qed.
 
-Lemma compute_sdom_chains__entry: forall f entry rd l0 chain0,
+Lemma gt_sdom_prop_entry: forall f l1 entry
+  (H: getEntryLabel f = ret entry)
+  (H4: gt_sdom_prop (bound_fdef f) (dom_analyze f) l1 entry),
+  False.
+Proof.
+  intros.
+  unfold gt_sdom_prop, gt_sdom in H4.
+  remember ((dom_analyze f) !! entry) as R.
+  destruct R.
+  assert (exists ps, exists cs, exists tmn, 
+    getEntryBlock f = Some (block_intro entry ps cs tmn)) as Hentry.
+    destruct f as [fh bs]. destruct bs; tinv H. 
+    destruct b; inv H; simpl; eauto.
+  destruct Hentry as [ps [cs [tmn Hentry]]].
+  apply dom_entrypoint in Hentry.
+  rewrite <- HeqR in Hentry. simpl in Hentry. subst.
+  inv H4.
+Qed.
+
+Lemma entry_in_compute_sdom_chains: forall entry l0 chain0 bd res rd
+  (H:forall b, b <> entry /\ In b rd -> 
+     match (AMap.get b res) with
+     | Dominators.mkBoundedSet dts _ => dts <> nil -> In entry dts
+     end)
+  (H0:In (l0, chain0) (compute_sdom_chains bd res rd))
+  (Huniq:NoDup chain0)
+  (G:(length chain0 > 1)%nat),
+  In entry chain0.
+Proof.
+  intros.
+  assert (H0':=H0).
+  apply compute_sdom_chains__dom in H0'.
+  remember (AMap.get l0 res) as R.
+  destruct R.
+  assert (H1':=H0).
+  eapply compute_sdom_chains_safe with (l1:=entry) in H0; eauto.
+  apply H0.
+  simpl.
+  destruct (l_dec l0 entry); subst; auto.
+    assert (l0 <> entry /\ In l0 rd) as J.
+      auto.
+    apply H in J. rewrite <- HeqR in J.
+    right. 
+    apply J.
+    destruct bs_contents.
+      destruct chain0; tinv G.      
+      destruct chain0; try solve [contradict G; simpl; clear; omega].
+      assert (H2':=H1').
+      eapply compute_sdom_chains_safe with (l1:=l1) in H1'; eauto.
+      eapply compute_sdom_chains_safe with (l1:=l2) in H2'; eauto.
+      assert (In l1 (l1 :: l2 :: chain0)) as Hin1. simpl. auto.
+      assert (In l2 (l1 :: l2 :: chain0)) as Hin2. simpl. auto.
+      apply H1' in Hin1.
+      apply H2' in Hin2.
+      simpl in Hin1, Hin2.
+      destruct Hin1; subst; try tauto.
+      destruct Hin2; subst; try tauto.
+      inv Huniq. contradict H3; simpl; auto.
+
+      congruence.
+Qed.
+
+Lemma dom_analysis__entry_doms_others2: forall ifs S M f 
+  (HwfF: wf_fdef ifs S M f) entry rd,
   getEntryLabel f = Some entry ->
-  reachablity_analysis f =  Some rd ->
-  In (l0, chain0)
-    (compute_sdom_chains
-      (dep_doms__nondep_doms (bound_fdef f) (dom_analyze f)) rd) ->
+  reachablity_analysis f = Some rd ->
+  (forall b, b <> entry /\ In b rd -> 
+     match (AMap.get b (dom_analyze f)) with
+     | Dominators.mkBoundedSet dts _ => dts <> nil -> In entry dts
+     end).
+Proof.
+  intros.
+  destruct H1 as [J1 J2].
+  case_eq ((dom_analyze f) !! b).
+  intros bs_contents bs_bound H1 Hnnil.
+  unfold dom_analyze in H1.
+  destruct f.
+  remember (entry_dom b0) as R.
+  destruct R. 
+  destruct x as [[]|]; subst.
+    destruct b0; inv H.
+    destruct b1; tinv y.
+    destruct bs_contents0; tinv y.
+    destruct b0. inv HeqR.
+    inv H3.
+    remember (
+      DomDS.fixpoint (bound_blocks (block_intro entry p c t :: b2))
+           (successors_blocks (block_intro entry p c t :: b2))
+           (transfer (bound_blocks (block_intro entry p c t :: b2)))
+           ((entry,
+            {| DomDS.L.bs_contents := nil; DomDS.L.bs_bound := bs_bound0 |})
+            :: nil)) as R.
+    destruct R.
+      symmetry in HeqR.
+      eapply EntryDomsOthers.dom_entry_doms_others with (entry:=entry) in HeqR; 
+        eauto.
+        unfold EntryDomsOthers.entry_doms_others in HeqR.
+        apply HeqR in J1.
+        unfold Dominators.member in J1.
+        unfold EntryDomsOthers.dt, EntryDomsOthers.bound, DomDS.dt, DomDS.L.t 
+          in J1. 
+        unfold Dominators.t in H1. simpl in J1, H1.
+        rewrite H1 in J1; auto.
+
+        split. 
+           remember (Kildall.successors_list
+             (EntryDomsOthers.predecessors (block_intro entry p c t :: b2)) 
+               entry) as R.
+           destruct R; auto.
+           assert (
+             In a 
+               (Kildall.successors_list
+                 (EntryDomsOthers.predecessors (block_intro entry p c t :: b2)) 
+               entry)) as Hin. rewrite <- HeqR0. simpl; auto.
+           apply Kildall.make_predecessors_correct' in Hin.
+           change (successors_blocks (block_intro entry p c t :: b2)) with
+             (successors (fdef_intro f (block_intro entry p c t :: b2))) in Hin.
+           apply successors__blockInFdefB in Hin.
+           destruct Hin as [ps0 [cs0 [tmn0 [G1 G2]]]].
+           eapply getEntryBlock_inv with (l3:=a)(a:=entry) in G2; simpl; eauto.
+           congruence.
+
+        split; auto.
+          exists{| DomDS.L.bs_contents := nil; DomDS.L.bs_bound := bs_bound0 |}.
+          simpl.
+          split; auto.
+            split; intros x Hin; auto.
+
+      rewrite AMap.gso in H1; auto.
+      rewrite AMap.gi in H1.
+      inv H1. contradict Hnnil; auto.
+
+    inv H.
+Qed.
+
+Lemma entry_is_head_of_compute_sdom_chains: forall ifs S M f 
+  (HwfF: wf_fdef ifs S M f) (Huniq: uniqFdef f) entry rd l0 chain0
+  (H:getEntryLabel f = Some entry)
+  (H0:reachablity_analysis f = Some rd)
+  (H1:In (l0, chain0)
+    (compute_sdom_chains (bound_fdef f) (dom_analyze f) rd))
+  (G:(length chain0 > 1)%nat),
   exists chain0', chain0 = entry :: chain0'.
-Admitted.
+Proof.
+  intros. 
+  assert (forall b, 
+    b <> entry /\ In b rd -> 
+    match (AMap.get b (dom_analyze f)) with
+    | Dominators.mkBoundedSet dts _ => dts <> nil -> In entry dts
+    end) as J.
+    eapply dom_analysis__entry_doms_others2; eauto.
+  assert (J0:=H0).
+  apply reachablity_analysis__in_bound in H0.
+  assert (forall x : atom, In x rd -> reachable f x) as W.
+    intros. eapply reachablity_analysis__reachable; eauto.
+  assert (J1:=H1).
+  eapply compute_sdom_chains_sorted in J1; eauto.
+  destruct J1 as [J1 J2].
+  assert (H1':=H1).
+  apply entry_in_compute_sdom_chains with (entry:=entry) in H1'; auto.
+  apply compute_sdom_chains__in_bound in H1; auto.
+  destruct chain0.
+    inv H1'.
 
-Lemma compute_sdom_chains__wf_chain: forall f l0 chain0 entry rd,
+    simpl in H1'.
+    destruct (l_dec l1 entry); subst; eauto.
+    destruct H1' as [Heq | H1']; subst.
+      congruence.
+
+      apply strict_Sorted_StronglySorted in J1; auto.
+        inv J1.
+        inv J2.    
+        eapply Forall_forall in H5; eauto.
+        apply gt_sdom_prop_entry in H5; tauto. 
+
+        intros.
+        eapply gt_sdom_prop_trans with (l2:=y); eauto.
+Qed.
+
+Lemma compute_sdom_chains__wf_chain: forall ifs S M f 
+  (HwfF: wf_fdef ifs S M f) (Huniq: uniqFdef f) l0 chain0 entry rd,
   getEntryLabel f = Some entry ->
   reachablity_analysis f =  Some rd ->
-  In (l0, chain0)
-    (compute_sdom_chains
-       (dep_doms__nondep_doms (bound_fdef f) (dom_analyze f)) rd) ->
+  In (l0, chain0) (compute_sdom_chains (bound_fdef f) (dom_analyze f) rd) ->
   wf_chain f (DT_node entry DT_nil) chain0.
 Proof.
   intros.
+  destruct chain0; simpl; auto.
+  destruct chain0; simpl; auto.
   assert (H1':=H1).
-  eapply compute_sdom_chains__entry in H1'; eauto.
+  eapply entry_is_head_of_compute_sdom_chains in H1';
+    simpl; try solve [eauto | omega].
   destruct H1' as [chain0' H1']; subst; simpl.
+  inv H1'.
   split; auto.
-    eapply compute_sdom_chains_sorted; eauto.
+    eapply compute_sdom_chains_sorted; 
+      eauto using reachablity_analysis__in_bound.
+      intros. eapply reachablity_analysis__reachable; eauto.
 Qed.
 
 Fixpoint in_children_roots child dts : bool :=
@@ -354,7 +1495,7 @@ match getEntryLabel f, reachablity_analysis f with
 | Some root, Some rd =>
     let dt := dom_analyze f in
     let b := bound_fdef f in
-    let chains := compute_sdom_chains (dep_doms__nondep_doms b dt) rd in
+    let chains := compute_sdom_chains b dt rd in
     Some (fold_left 
       (fun acc elt => let '(_, chain):=elt in create_dtree_from_chain acc chain) 
       chains (DT_node root DT_nil))
@@ -799,7 +1940,7 @@ Lemma create_dtree__wf_dtree: forall f dt,
   | Some root, Some rd =>
       let dt' := dom_analyze f in
       let b := bound_fdef f in
-      let chains := compute_sdom_chains (dep_doms__nondep_doms b dt') rd in
+      let chains := compute_sdom_chains b dt' rd in
       forall p0 ch0,
         (is_dtree_edge dt p0 ch0 -> 
          exists l0, exists chain0, 
@@ -819,8 +1960,7 @@ Proof.
   destruct R; inv H.
   intros.
   destruct (@fold_left_create_dtree_from_chain__is_dtree_edge__is_chain_edge
-    p0 ch0 (compute_sdom_chains
-             (dep_doms__nondep_doms (bound_fdef f) (dom_analyze f)) l1)
+    p0 ch0 (compute_sdom_chains (bound_fdef f) (dom_analyze f) l1)
     (DT_node l0 DT_nil)) as [J1 J2].
   split; intros J; auto.
     apply J1 in J.
@@ -828,39 +1968,40 @@ Proof.
       simpl in J. destruct (id_dec p0 l0); tinv J.
 Qed.
 
-Fixpoint find_idom_aux (res: AMap.t (set l)) (acc:l) (dts: set l): option l :=
+Fixpoint find_idom_aux bd (res: AMap.t (Dominators.t bd)) (acc:l) (dts: set l)
+  : option l :=
 match dts with
 | nil => Some acc
 | l0::dts' =>
     match AMap.get l0 res, AMap.get acc res with
-    | dts1, dts2 =>
+    | Dominators.mkBoundedSet dts1 _ , Dominators.mkBoundedSet dts2 _ =>
         if (in_dec l_dec l0 dts2)
         then (* acc << l0 *)
-          find_idom_aux res acc dts' 
+          find_idom_aux bd res acc dts' 
         else
           if (in_dec l_dec acc dts1)
           then (* l0 << acc *)
-            find_idom_aux res l0 dts' 
+            find_idom_aux bd res l0 dts' 
           else (* l0 and acc are incompariable *)
             None
     end
 end.
 
 (* We should prove that this function is not partial. *)
-Definition find_idom (res: AMap.t (set l)) (l0:l) : option l :=
+Definition find_idom bd (res: AMap.t (Dominators.t bd)) (l0:l) : option l :=
 match AMap.get l0 res with
-| l1::dts0 => find_idom_aux res l1 dts0
+| Dominators.mkBoundedSet (l1::dts0) _ => find_idom_aux bd res l1 dts0
 | _ => None
 end.
 
-Fixpoint compute_idoms (res: AMap.t (set l)) (bd: list l) (acc: list (l * l)) :
-  list (l * l) :=
-match bd with
+Fixpoint compute_idoms bd (res: AMap.t (Dominators.t bd)) (rd: list l) 
+  (acc: list (l * l)) : list (l * l) :=
+match rd with
 | nil => acc
-| l0 :: bd' =>
-    match find_idom res l0 with
-    | None => compute_idoms res bd' acc
-    | Some l1 => compute_idoms res bd' ((l1,l0)::acc)
+| l0 :: rd' =>
+    match find_idom bd res l0 with
+    | None => compute_idoms bd res rd' acc
+    | Some l1 => compute_idoms bd res rd' ((l1,l0)::acc)
     end
 end.
 
