src/Transforms/gvn.v
@@ -667,28 +667,28 @@ end.
    id1 = r in l1 
 *)
 Fixpoint lookup_predundant_exp_for_id (f:fdef) (ndom: list l) 
-  (res: AMap.t (set l)) (l1:l) (r:rhs) : option (l * cmd) :=
+  bd (res: AMap.t (Dominators.t bd)) (l1:l) (r:rhs) : option (l * cmd) :=
 match ndom with
 | nil => None
 | l0::ndom' =>
     match (AMap.get l0 res) with
-    | dts0 =>
+    | Dominators.mkBoundedSet dts0 _ =>
       if (in_dec eq_atom_dec l1 dts0) then
-        lookup_predundant_exp_for_id f ndom' res l1 r
+        lookup_predundant_exp_for_id f ndom' bd res l1 r
       else
         match lookupBlockViaLabelFromFdef f l0 with
         | None => None
         | Some (block_intro _ _ cs _) =>
             match lookup_predundant_exp_from_cmds cs r with
-            | None => lookup_predundant_exp_for_id f ndom' res l1 r
+            | None => lookup_predundant_exp_for_id f ndom' bd res l1 r
             | Some c0 => Some (l0, c0)
             end
         end
     end
 end.
 
-Fixpoint lookup_predundant_exp (f:fdef) (res: AMap.t (set l)) (rd0 rd:list l) 
-  : option (l * id * l * cmd) :=
+Fixpoint lookup_predundant_exp (f:fdef) bd (res: AMap.t (Dominators.t bd)) 
+  (rd0 rd:list l) : option (l * id * l * cmd) :=
 match rd with
 | nil => None
 | l1::rd' =>
@@ -696,7 +696,7 @@ match rd with
     | None => None
     | Some (block_intro _ _ cs _) =>
         match (AMap.get l1 res) with
-        | dts1 =>
+        | Dominators.mkBoundedSet dts1 _ =>
            let ndom := 
              ListSet.set_diff id_dec 
                (ListSet.set_inter id_dec rd0 (bound_fdef f)) (l1::dts1) in
@@ -708,7 +708,7 @@ match rd with
                           | Some id1 =>
                               if pure_cmd c then
                                 match 
-                                  lookup_predundant_exp_for_id f ndom res l1  
+                                  lookup_predundant_exp_for_id f ndom bd res l1
                                     (rhs_of_cmd c) with
                                 | Some (l0, c0) => Some (l1, id1, l0, c0)
                                 | None => None
@@ -718,26 +718,27 @@ match rd with
                           end
                         | _ => acc
                         end) cs None with
-           | None => lookup_predundant_exp f res rd0 rd'
+           | None => lookup_predundant_exp f bd res rd0 rd'
            | Some re => Some re
            end
         end
     end
 end.
 
-Definition find_gcd_dom (res: AMap.t (set l)) (l1 l2:l) : option l :=
+Definition find_gcd_dom bd (res: AMap.t (Dominators.t bd)) (l1 l2:l): option l:=
 match AMap.get l1 res, AMap.get l2 res with
-| dts1, dts2 =>
+| Dominators.mkBoundedSet dts1 _, Dominators.mkBoundedSet dts2 _ =>
   match ListSet.set_inter id_dec dts1 dts2 with
-  | l0::dts0 => find_idom_aux res l0 dts0
+  | l0::dts0 => find_idom_aux bd res l0 dts0
   | _ => None
   end
 end.
 
-Definition pre_fdef (f:fdef) (res: AMap.t (set l)) (rd:list l) : fdef * bool :=
-match lookup_predundant_exp f res rd rd with
+Definition pre_fdef (f:fdef) bd (res: AMap.t (Dominators.t bd)) (rd:list l) 
+  : fdef * bool :=
+match lookup_predundant_exp f bd res rd rd with
 | Some (l1, id1, l0, c0) =>
-    match find_gcd_dom res l1 l0 with
+    match find_gcd_dom _ res l1 l0 with
     | Some l2 =>
         match lookupBlockViaLabelFromFdef f l2 with
         | None => (f, false)
@@ -753,18 +754,18 @@ end.
 
 Parameter does_pre : unit -> bool.
 
-Definition opt_step (dt:DTree) (res: AMap.t (set l)) (rd:list l) (f: fdef)
-  : fdef + fdef :=
+Definition opt_step (dt:DTree) bd (res: AMap.t (Dominators.t bd )) (rd:list l) 
+  (f: fdef) : fdef + fdef :=
 let '(f1, changed1) := gvn_fdef_dtree f false nil dt in
 if changed1 then inr _ f1 
 else 
   if does_pre tt then
-    let '(f2, changed2) := pre_fdef f1 res rd in
+    let '(f2, changed2) := pre_fdef f1 bd res rd in
     if changed2 then inr _ f2 else inl _ f2
   else inl _ f1.
 
 Parameter print_reachablity : list l -> bool.
-Parameter print_dominators : list l -> AMap.t (set l) -> bool.
+Parameter print_dominators : forall bd, AMap.t (Dominators.t bd) -> bool.
 Parameter print_dtree : DTree -> bool.
 
 Definition dce_block (f:fdef) (b:block) : fdef :=
@@ -795,8 +796,8 @@ Definition opt_fdef (f:fdef) : fdef :=
 match getEntryBlock f, reachablity_analysis f with
 | Some (block_intro root _ _ _), Some rd =>
     let b := bound_fdef f in
-    let dts := dep_doms__nondep_doms b (dom_analyze f) in
-    let chains := compute_sdom_chains dts rd in
+    let dts := dom_analyze f in
+    let chains := compute_sdom_chains b dts rd in
     let dt :=
       fold_left 
       (fun acc elt => 
@@ -806,7 +807,7 @@ match getEntryBlock f, reachablity_analysis f with
     if print_reachablity rd && print_dominators b dts && 
        print_dtree dt && read_aa_from_fun (getFdefID f) then
        match fix_temporary_fdef 
-               (SafePrimIter.iterate _ (opt_step dt dts rd) 
+               (SafePrimIter.iterate _ (opt_step dt b dts rd) 
                  (dce_fdef f)) with
        | Some f' => f'
        | _ => f
